change precondition handling to use classes

src/ProofOfConcept/Candidates.v
@@ -1,20 +1,22 @@
+Require Import Coq.ZArith.ZArith.
 Require Import Coq.micromega.Lia.
 Require Import Coq.Lists.List.
 Require Import Optimizer.Machine.
 Require Import Optimizer.ProofOfConcept.Enumerators.
-Require Import Optimizer.ProofOfConcept.Glue.
 Require Import Optimizer.ProofOfConcept.Instructions.
 Require Import Optimizer.ProofOfConcept.Registers.
+Require Import Optimizer.ProofOfConcept.Glue.
+Import Machine.
+Local Open Scope Z_scope.
 
 Module All.
   Definition rep (ap : abstract_program) (p : program) : Prop := to_abstract p = ap.
-  Definition rep_enum :=
-    (enumerate_concrete Instructions.instr_size Instructions.num_source_regs Registers.all_registers).
+  Definition rep_enum := (enumerate_concrete instr_size).
   Lemma rep_enum_complete t p : valid p -> rep t p -> In p (rep_enum t).
   Proof.
     cbv [rep rep_enum]. intros; subst.
-    eapply enumerate_concrete_complete;
-      eauto using all_registers_complete, precondition_length_args, precondition_instr_size.
+    eapply enumerate_concrete_complete; eauto;
+      apply precondition_length_args || apply precondition_instr_size.
   Qed.
   Lemma rep_enum_sound t p : In p (rep_enum t) -> rep t p.
   Proof.
@@ -23,8 +25,7 @@ Module All.
     reflexivity.
   Qed.
 
-  Definition candidates p :=
-    enumerate_under_cost Instructions.instr_cost Instructions.all_instructions (cost p).
+  Definition candidates p := enumerate_under_cost instr_cost (cost p).
   Lemma candidates_complete p_spec op :
     optimal op ->
     equivalent p_spec op ->
@@ -33,21 +34,18 @@ Module All.
       rep t op /\ In t (candidates p_spec).
   Proof.
     intros. exists (to_abstract op).
-    split; [reflexivity|].
-    cbv [candidates].
-    apply enumerate_under_cost_complete with (cost:=cost);
-      auto using instr_cost_pos, all_instructions_complete.
+    split; [reflexivity|]. cbv [candidates].
+    eapply enumerate_under_cost_complete;
+      eauto using instr_cost_pos, all_instructions_complete.
     intros; cbn; lia.
   Qed.
 
-  Notation optimal_limited_domain_equiv :=
-    (fun p valid_p =>
-       optimal_limited_domain_equiv rep
-                                    rep_enum
-                                    rep_enum_complete
-                                    rep_enum_sound
-                                    p
-                                    valid_p
-                                    (candidates p)
-                                    (candidates_complete p)).
+  Lemma optimal_limited_domain_equiv p_spec :
+    valid p_spec ->
+    Forall (fun ap => forall p' : program, rep ap p' -> valid p' -> ~ p_spec == p') (candidates p_spec) ->
+    optimal p_spec.
+  Proof.
+    intros. pose proof (optimal_limited_domain_equiv rep).
+    eauto using rep_enum_complete, rep_enum_sound, candidates_complete.
+  Qed.
 End All.
