src/ProofOfConcept/CostModel.v
@@ -1,28 +1,24 @@
 Require Import Coq.ZArith.ZArith.
 Require Import Coq.Lists.List.
 Require Import Optimizer.Machine.
+Require Import Optimizer.System.
 
 Module CostModel.
   Import Machine.
   Section CostModel.
-    Context {register flag instruction : Set}
-            {register_size : register -> Z}
-            {instr_cost : instruction -> nat}
-            {precondition : instruction -> register -> list (register + Z) -> Prop}.
-    Local Notation program := (Machine.program (register:=register) (instruction:=instruction)).
-    Local Notation valid := (Machine.valid (precondition:=precondition)).
-    Context (equivalent : program -> program -> Prop).
-
+    Context `{instrt : instr_impl} {instr_cost : instruction -> nat}.
     Fixpoint cost (p : program) : nat :=
       match p with
       | Ret r => 0
       | Instr i rd args cont => i.(instr_cost) + cost cont
       end.
 
-    Definition optimal (p : program) : Prop :=
-      forall p' : program,
-        valid p'
-        -> (equivalent p p')
-        -> (cost p <= cost p')%nat.
+    Section Proofs.
+      Context (instr_cost_pos : forall i, (0 < instr_cost i)%nat).
+
+      Lemma cost_of_instr_pos i rd args cont :
+        (cost cont < cost (Machine.Instr i rd args cont))%nat.
+      Proof. specialize (instr_cost_pos i). cbn [cost]. omega. Qed.
+    End Proofs.
   End CostModel.
 End CostModel.
