src/ProofOfConcept/Glue.v
@@ -1,70 +1,98 @@
 Require Import Coq.ZArith.ZArith.
 Require Import Optimizer.Machine.
+Require Import Optimizer.System.
 Require Import Optimizer.ProofOfConcept.CostModel.
 Require Import Optimizer.ProofOfConcept.Flags.
-Require Import Optimizer.ProofOfConcept.Instructions.
 Require Import Optimizer.ProofOfConcept.Optimality.
 Require Import Optimizer.ProofOfConcept.Maps.
 Require Import Optimizer.ProofOfConcept.Registers.
+Require Optimizer.ProofOfConcept.Instructions.
 Local Open Scope Z_scope.
-Import Maps.
 
-Notation exec := (Machine.exec
-                    (register_size:=Registers.size)
-                    (flag_spec:=Flags.flag_spec)
-                    (flags_written:=Instructions.flags_written)
-                    (spec:=Instructions.spec)).
-Notation precondition :=
-  (Instructions.precondition (register_size:=Registers.size)).
-Notation valid := (Machine.valid
-                     (register:=Registers.register)
-                     (precondition:=precondition)).
-Notation program := (Machine.program
-                       (register:=Registers.register)
-                       (instruction:=Instructions.instruction)).
-Notation valid_context := (Machine.valid_context
-                             (register:=Registers.register)
-                             (register_size:=Registers.size)).
-Notation equivalent := (Machine.equivalent
-                          (register_size:=Registers.size)
-                          (flag_spec := Flags.flag_spec)
-                          (flags_written := Instructions.flags_written)
-                          (spec := Instructions.spec)).
-Infix "==" := equivalent (at level 40).
+Instance regt : reg_impl :=
+  {|
+    register := Registers.register;
+    reg_mapt := Maps.RegMaps.reg_mapt;
+    reg_enum := {|
+                 enum := Registers.all_registers;
+                 enum_complete := all_registers_complete;
+               |};
+    register_size := Registers.size;
+    reg_eq_dec := Registers.reg_eq_dec
+  |}.
+Instance flagt : flag_impl :=
+  {|
+    flag := Flags.flag;
+    flag_mapt := Maps.FlagMaps.flag_mapt;
+    flag_enum := {|
+                  enum := Flags.all_flags;
+                  enum_complete := all_flags_complete
+                |};
+    flag_spec := Flags.flag_spec;
+    flag_eq_dec := Flags.flag_eq_dec;
+  |}.
+Instance instrt : instr_impl :=
+  {|
+    instruction := Instructions.instruction;
+    instr_enum := {|
+                   enum := Instructions.all_instructions;
+                   enum_complete := Instructions.all_instructions_complete;
+                 |};
+    flags_written := Instructions.flags_written;
+    num_source_regs := Instructions.num_source_regs;
+    spec := Instructions.spec;
+    precondition := Instructions.precondition (register_size:=Registers.size);
+    instr_eq_dec := Instructions.instr_eq_dec;
+    precondition_dec := Instructions.precondition_dec;
+  |}.
+
 Notation cost := (CostModel.cost
-                    (register:=Registers.register)
                     (instr_cost:=Instructions.instr_cost)).
-Notation optimal := (CostModel.optimal
-                       (instr_cost:=Instructions.instr_cost)
-                       (precondition:=precondition)
-                       equivalent).
-
-(* TODO: make this rely on fewer things (for instance, parameterize over [equivalent]) *)
+Notation optimal := (Optimality.optimal cost).
+Lemma instr_cost_eq i rd args cont :
+  cost (Machine.Instr i rd args cont) = (cost cont + Instructions.instr_cost i)%nat.
+Proof. cbn [CostModel.cost]. omega. Qed.
+Lemma ret_cost_eq r : cost (Machine.Ret r) = 0%nat.
+Proof. reflexivity. Qed.
 Notation optimal_limited_domain_equiv :=
   (Optimality.optimal_limited_domain_equiv
-     reg_map_equiv
-     flag_map_equiv
-     Instructions.instr_size
-     Registers.size
-     Instructions.instr_cost
-     Instructions.num_source_regs
-     precondition
-     Flags.flag_spec
-     Instructions.flags_written
-     Instructions.spec
-     Flags.flag_eq_dec
-     Registers.reg_eq_dec
-     Instructions.instr_eq_dec
-     (fun m1 m2 => reg_map_dec m1 m2 Z.eq_dec)
-     (fun m1 m2 => flag_map_dec m1 m2 Bool.bool_dec)
-     Flags.all_flags
-     Registers.all_registers
-     Instructions.all_instructions
-     all_flags_complete
-     all_registers_complete
-     all_instructions_complete
-     instr_cost_pos
-     precondition_instr_size
-     precondition_length_args
-     precondition_dec
+     cost
+     (CostModel.cost_of_instr_pos Instructions.instr_cost_pos)
+     (Enumerators.enumerate_programs_under_cost Instructions.instr_cost Instructions.instr_size)
+     (Enumerators.enumerate_under_cost_with_condition Instructions.instr_cost Instructions.instr_size)
+     (Enumerators.enumerate_programs_under_cost_complete_alt
+        Instructions.instr_cost
+        Instructions.instr_size
+        cost
+        Instructions.instr_cost_pos
+        instr_cost_eq
+        Instructions.precondition_instr_size
+        Instructions.precondition_length_args)
+     (Enumerators.enumerate_under_cost_with_condition_complete
+        Instructions.instr_cost
+        Instructions.instr_size
+        cost
+        Instructions.instr_cost_pos
+        instr_cost_eq
+        Instructions.precondition_instr_size
+        Instructions.precondition_length_args)
+     (Enumerators.enumerate_under_cost_with_condition_sound
+        Instructions.instr_cost
+        Instructions.instr_size)
+     (Enumerators.enumerate_under_cost_with_condition_bound
+        Instructions.instr_cost
+        Instructions.instr_size
+        cost
+        Instructions.instr_cost_pos
+        ret_cost_eq
+        instr_cost_eq
+     )
+     (Enumerators.enumerate_under_cost_with_condition_zero
+        Instructions.instr_cost
+        Instructions.instr_size)
+     Enumerators.enumerate_contexts
+     (Enumerators.enumerate_contexts_complete Maps.reg_map_equiv)
+     Maps.flag_map_equiv
+     (fun m1 m2 => Maps.reg_map_dec m1 m2 Z.eq_dec)
+     (fun m1 m2 => Maps.flag_map_dec m1 m2 Bool.bool_dec)
   ).
