src/System.v
@@ -1,0 +1,61 @@
+Require Import Coq.ZArith.ZArith.
+Require Import Coq.Lists.List.
+Require Import Optimizer.AbstractMap.
+
+Class enumerator T :=
+  {
+    enum : list T;
+    enum_complete : forall t : T, In t enum;
+  }.
+Hint Resolve @enum_complete.
+
+Class reg_impl :=
+  {
+    register : Type;
+    reg_mapt : map_impl register;
+    reg_enum : enumerator register;
+    register_size : register -> Z;
+    reg_eq_dec : forall r1 r2 : register, {r1 = r2} + {r1 <> r2};
+  }.
+
+Class flag_impl :=
+  {
+    flag : Type;
+    flag_mapt : map_impl flag;
+    flag_enum : enumerator flag;
+    flag_spec : Z (* destination register size *) -> flag -> Z -> bool;
+    flag_eq_dec : forall f1 f2 : flag, {f1 = f2} + {f1 <> f2};
+  }.
+
+Class instr_impl {regt : reg_impl} {flagt : flag_impl} :=
+  {
+    instruction : Type;
+    instr_enum : enumerator instruction;
+    flags_written : instruction -> list (@flag flagt);
+    num_source_regs : instruction -> nat;
+    spec : instruction -> list Z -> (@flag flagt -> bool) -> Z;
+    precondition : instruction -> @register regt -> list (@register regt + Z) -> Prop;
+    instr_eq_dec : forall i1 i2 : instruction, {i1 = i2} + {i1 <> i2};
+    precondition_dec : forall i rd args, {precondition i rd args} + {~ precondition i rd args};
+  }.
+
+(*
+(* TODO: not currently in use because maps are not abstract state yet *)
+Class machine_impl :=
+  {
+    state : Type;
+    program : Type;
+    valid : program -> Prop;
+    valid_state : state -> Prop;
+    exec : program -> state -> state;
+    equivalent : program -> program -> Prop;
+    valid_dec : forall p, {valid p} + {~ valid p};
+    equiv_dec : forall p1 p2, {equivalent p1 p2} + {~ equivalent p1 p2};
+    program_eq_dec : forall p1 p2 : program, {p1 = p2} + {p1 <> p2};
+    (*
+    (* TODO: this seems like maybe a natural property to want *)
+    exec_preserves_valid :
+      forall s p, valid_state s -> valid p -> valid_state (exec p s)
+     *)
+  }.
+*)
